src/tree/layer2/UnorderedSetArrayList.dfy
@@ -1,0 +1,156 @@
+include "../../../src/tree/layer1/UnorderedSet.dfy"
+include "../../../src/tree/layer1/OrderedSetUtils.dfy"
+
+
+
+
+
+
+trait UnorderedSetArrayList extends UnorderedSet {
+
+
+  method contains(x:int) returns (b:bool)
+   modifies this, Repr()
+   requires Valid()
+   requires forall x | x in Repr() :: allocated(x)
+   ensures Valid() && Model()==old(Model())
+   ensures b==(x in Model())
+   
+   ensures forall x {:trigger x in Repr(), x in old(Repr())} | x in Repr() - old(Repr()) :: fresh(x)
+   ensures fresh(Repr()-old(Repr()))
+   ensures forall x | x in Repr() :: allocated(x)
+   
+   ensures Iterators() == old(Iterators())
+   ensures forall it | it in old(Iterators()) && old(it.Valid()) ::
+      it.Valid() && 
+      it.Traversed() == old(it.Traversed()) && 
+      (it.HasNext() ==> it.Peek()==old(it.Peek()))
+
+ 
+  
+
+  method add(x:int)
+    modifies this,Repr()
+    requires Valid()
+    requires forall x | x in Repr() :: allocated(x)
+    ensures Valid()
+    ensures Model() == old(Model()) + {x} 
+
+    ensures forall x {:trigger x in Repr(), x in old(Repr())} | x in Repr() - old(Repr()) :: fresh(x)
+    ensures fresh(Repr()-old(Repr()))
+    ensures forall x | x in Repr() :: allocated(x)
+   
+    ensures Iterators() == old(Iterators())
+    ensures forall it | it in old(Iterators()) && old(it.Valid()) ::
+      it.Valid() && 
+      it.Traversed() == old(it.Traversed()) &&
+      (it.HasNext() ==> (if (it.Traversed()!=old(Model())) 
+                          then it.Peek()==old(it.Peek())
+                          else it.Peek()==x))
+
+
+
+  method remove(x:int) 
+    modifies this,Repr()
+    requires Valid()
+    requires forall x | x in Repr() :: allocated(x)
+    ensures Valid()
+    ensures Model()== old(Model()) - {x} 
+
+    ensures forall x {:trigger x in Repr(), x in old(Repr())} | x in Repr() - old(Repr()) :: fresh(x)
+    ensures fresh(Repr()-old(Repr()))
+    ensures forall x | x in Repr() :: allocated(x)
+
+    ensures Iterators() == old(Iterators())
+    ensures forall it | it in old(Iterators()) && old(it.Valid()) && old(it.HasNext())  ::
+      it.Valid() && 
+      if (x !in old(it.Traversed())) then  
+           it.Traversed()==old(it.Traversed()) && (it.HasNext() && old(it.Peek())!=x ==> it.Peek()==old(it.Peek()))
+      else      
+           it.Traversed() == old(it.Traversed())+{old(it.Peek())}-{x}
+
+    
+
+  method find(x:int) returns (newt:UnorderedSetIterator)
+    modifies this, Repr()
+    requires Valid()
+    requires forall x | x in Repr() :: allocated(x)
+    ensures Valid() 
+    ensures Model()==old(Model())
+    
+    ensures fresh(newt) 
+    ensures newt.Valid() && newt.Parent()==this
+    ensures x in old(Model()) ==> newt.HasNext() && newt.Peek()==x
+    ensures x !in old(Model()) ==> newt.Traversed()==Model()
+
+    ensures forall x {:trigger x in Repr(), x in old(Repr())} | x in Repr() - old(Repr()) :: fresh(x)
+    ensures fresh(Repr()-old(Repr()))
+    ensures forall x | x in Repr() :: allocated(x)
+
+    ensures Iterators() == {newt}+old(Iterators())
+    ensures forall it | it in old(Iterators()) && old(it.Valid()) ::
+      it.Valid() && 
+      it.Traversed() == old(it.Traversed()) &&
+      (it.HasNext() ==> it.Peek()==old(it.Peek()))
+
+  
+
+  method insert(mid: UnorderedSetIterator, x: int) returns (newt:UnorderedSetIterator)
+    modifies this, Repr()
+    requires Valid()
+    requires mid.Valid() 
+    requires mid.Parent() == this
+    requires mid in Iterators()
+    requires forall x | x in Repr() :: allocated(x)
+    ensures Valid()
+    ensures Model() == old(Model()) + {x}
+
+    ensures fresh(newt)
+    ensures Iterators() == {newt}+old(Iterators())
+    ensures newt.Valid() && newt.Parent()==this  
+    ensures newt.HasNext() && newt.Peek()==x 
+
+    ensures forall x {:trigger x in Repr(), x in old(Repr())} | x in Repr() - old(Repr()) :: fresh(x)
+    ensures fresh(Repr()-old(Repr()))
+    ensures forall x | x in Repr() :: allocated(x)
+  
+    ensures forall it | it in old(Iterators()) && old(it.Valid()) ::
+      it.Valid() && 
+      it.Traversed() == old(it.Traversed()) &&
+      (it.HasNext() ==> (if (it.Traversed()!=old(Model())) 
+                          then it.Peek()==old(it.Peek())
+                          else it.Peek()==x))
+
+
+
+
+  method erase(mid:UnorderedSetIterator) returns (next: UnorderedSetIterator)
+    modifies this, Repr()
+    requires Valid()
+    requires mid.Valid()
+    requires mid.Parent() == this
+    requires mid.HasNext()
+    requires mid in Iterators()
+    requires forall x | x in Repr() :: allocated(x)
+    ensures Valid()
+    ensures Model()== old(Model())-{old(mid.Peek())}
+    
+    ensures fresh(next)
+    ensures Iterators() == {next}+old(Iterators())
+    ensures next.Valid() && next.Parent()==this 
+    ensures next.Traversed()==old(mid.Traversed()) 
+
+    ensures forall x {:trigger x in Repr(), x in old(Repr())} | x in Repr() - old(Repr()) :: fresh(x)
+    ensures fresh(Repr()-old(Repr()))
+    ensures forall x | x in Repr() :: allocated(x)
+
+    ensures forall it | it in old(Iterators()) && old(it.Valid()) && old(it.HasNext())  ::
+      it.Valid() && 
+      if (old(mid.Peek()) !in old(it.Traversed())) then  
+           it.Traversed()==old(it.Traversed()) && (it.HasNext() && old(it.Peek())!=old(mid.Peek()) ==> it.Peek()==old(it.Peek()))
+      else      
+           it.Traversed() == old(it.Traversed())+{old(it.Peek())}-{old(mid.Peek())}
+
+}
+
+
